# baseURI: https://periodo.github.io/edtf-literals/draft

@prefix : <https://periodo.github.io/edtf-literals/draft/> .
@prefix dct: <http://purl.org/dc/terms/> .
@prefix greg: <http://www.w3.org/ns/time/gregorian/> .
@prefix owl: <http://www.w3.org/2002/07/owl#> .
@prefix rdf: <http://www.w3.org/1999/02/22-rdf-syntax-ns#> .
@prefix rdfs: <http://www.w3.org/2000/01/rdf-schema#> .
@prefix skos: <http://www.w3.org/2004/02/skos/core#> .
@prefix time: <http://www.w3.org/2006/time#> .
@prefix xsd: <http://www.w3.org/2001/XMLSchema#> .

<https://periodo.github.io/edtf-literals/draft>
  a owl:Ontology ;
  dct:creator <https://orcid.org/0000-0002-5486-159X> ;
  rdfs:comment "Draft ontology for EDTF concepts."@en ;
  rdfs:label "Extended Date/Time Format (EDTF) concepts"@en ;
  owl:imports <http://www.w3.org/2006/time>
  .

:unitSeason
  a time:TemporalUnit ;
  rdfs:label "Season (unit of temporal duration)"@en ;
  skos:prefLabel "season"@en
  .

:unitQuarter
  a time:TemporalUnit ;
  rdfs:label "Quarter (unit of temporal duration equivalent to 3 months)"@en ;
  skos:prefLabel "quarter"@en ;
  time:days "0"^^xsd:decimal ;
  time:hours "0"^^xsd:decimal ;
  time:minutes "0"^^xsd:decimal ;
  time:months "3"^^xsd:decimal ;
  time:seconds "0"^^xsd:decimal ;
  time:weeks "0"^^xsd:decimal ;
  time:years "0"^^xsd:decimal
  .

:unitQuadrimester
  a time:TemporalUnit ;
  rdfs:label "Quadrimester (unit of temporal duration equivalent to 4 months)"@en ;
  skos:prefLabel "quadrimester"@en ;
  time:days "0"^^xsd:decimal ;
  time:hours "0"^^xsd:decimal ;
  time:minutes "0"^^xsd:decimal ;
  time:months "4"^^xsd:decimal ;
  time:seconds "0"^^xsd:decimal ;
  time:weeks "0"^^xsd:decimal ;
  time:years "0"^^xsd:decimal
  .

:unitSemestral
  a time:TemporalUnit ;
  rdfs:label "Semestral (unit of temporal duration equivalent to 6 months)"@en ;
  skos:prefLabel "semestral"@en ;
  time:days "0"^^xsd:decimal ;
  time:hours "0"^^xsd:decimal ;
  time:minutes "0"^^xsd:decimal ;
  time:months "6"^^xsd:decimal ;
  time:seconds "0"^^xsd:decimal ;
  time:weeks "0"^^xsd:decimal ;
  time:years "0"^^xsd:decimal
  .

:YearSubdivision
  a owl:Class ;
  rdfs:comment "A subdivision of the year"@en ;
  rdfs:label "Subdivision of year"@en ;
  rdfs:subClassOf owl:Thing ;
  skos:definition "A subdivision of the year"@en ;
  skos:note "Membership of the class :YearSubdivision is open, to allow for alternative subdivisions."@en
  .

:Season
  a owl:Class ;
  rdfs:comment "A season of the year"@en ;
  rdfs:label "Season of year"@en ;
  rdfs:subClassOf :YearSubdivision ;
  rdfs:subClassOf [
      a owl:Restriction ;
      owl:hasValue :unitSeason ;
      owl:onProperty time:unitType ;
    ] ;
  skos:definition "A season of the year"@en ;
  skos:note "Membership of the class :Season is open, to allow for alternative seasons."@en
  .

:Quarter
  a owl:Class ;
  rdfs:comment "A quarter of the year"@en ;
  rdfs:label "Quarter of year"@en ;
  rdfs:subClassOf :YearSubdivision ;
  rdfs:subClassOf [
      a owl:Restriction ;
      owl:hasValue :unitQuarter ;
      owl:onProperty time:unitType ;
    ] ;
  owl:oneOf (
    :Quarter1
    :Quarter2
    :Quarter3
    :Quarter4
    ) ;
  skos:definition "A quarter of the year"@en
  .

:Quadrimester
  a owl:Class ;
  rdfs:comment "A quadrimester of the year"@en ;
  rdfs:label "Quadrimester of year"@en ;
  rdfs:subClassOf :YearSubdivision ;
  rdfs:subClassOf [
      a owl:Restriction ;
      owl:hasValue :unitQuadrimester ;
      owl:onProperty time:unitType ;
    ] ;
  owl:oneOf (
    :Quadrimester1
    :Quadrimester2
    :Quadrimester3
    ) ;
  skos:definition "A quadrimester of the year"@en
  .

:Semestral
  a owl:Class ;
  rdfs:comment "A semestral of the year"@en ;
  rdfs:label "Semestral of year"@en ;
  rdfs:subClassOf :YearSubdivision ;
  rdfs:subClassOf [
      a owl:Restriction ;
      owl:hasValue :unitSemestral ;
      owl:onProperty time:unitType ;
    ] ;
  owl:oneOf (
    :Semestral1
    :Semestral2
    ) ;
  skos:definition "A semestral of the year"@en
  .

:uncertainTemporalPosition
  rdf:type owl:ObjectProperty ;
  rdfs:comment "Uncertain position of a time instant"@en ;
  rdfs:domain time:Instant ;
  rdfs:label "Uncertain temporal position"@en ;
  rdfs:range time:TemporalPosition ;
  rdfs:subPropertyOf time:inTemporalPosition ;
  skos:definition "Uncertain position of a time instant"@en ;
  .

:approximateTemporalPosition
  rdf:type owl:ObjectProperty ;
  rdfs:comment "Approximate position of a time instant"@en ;
  rdfs:domain time:Instant ;
  rdfs:label "Approximate temporal position"@en ;
  rdfs:range time:TemporalPosition ;
  rdfs:subPropertyOf time:inTemporalPosition ;
  skos:definition "Approximate position of a time instant"@en ;
  .

:uncertainApproximateTemporalPosition
  rdf:type owl:ObjectProperty ;
  rdfs:comment "Uncertain and approximate position of a time instant"@en ;
  rdfs:domain time:Instant ;
  rdfs:label "Uncertain and approximate temporal position"@en ;
  rdfs:range time:TemporalPosition ;
  rdfs:subPropertyOf :uncertainTemporalPosition ;
  rdfs:subPropertyOf :approximateTemporalPosition ;
  skos:definition "Uncertain and approximate position of a time instant"@en ;
  .

:yearSubdivision
  a owl:ObjectProperty ;
  rdfs:comment "The subdivision of the year, whose value is a member of the class edtfo:YearSubdivision"@en ;
  rdfs:domain :SubYearDateDescription ;
  rdfs:label "year subdivision"@en ;
  rdfs:range :YearSubdivision ;
  skos:definition "The subdivision of the year, whose value is a member of the class edtfo:YearSubdivision"@en ;
  .

:SubYearDateDescription
  a owl:Class ;
  rdfs:comment "Description of date structured with separate values for year and a sub-year grouping such as a season or quarter. The temporal reference system is fixed to Gregorian Calendar and the range of the year property is restricted to xsd:gYear."@en ;
  rdf:label "Sub-year date description"@en ;
  rdfs:subClassOf time:TemporalPosition ;
  rdfs:subClassOf [
      a owl:Restriction ;
      owl:cardinality "1"^^xsd:nonNegativeInteger ;
      owl:onProperty time:unitType ;
    ] ;
  rdfs:subClassOf [
      a owl:Restriction ;
      owl:cardinality "1"^^xsd:nonNegativeInteger ;
      owl:onProperty :yearSubdivision ;
    ] ;
  rdfs:subClassOf [
      a owl:Restriction ;
      owl:cardinality "1"^^xsd:nonNegativeInteger ;
      owl:onProperty time:year ;
    ] ;
  rdfs:subClassOf [
      a owl:Restriction ;
      owl:allValuesFrom xsd:gYear ;
      owl:onProperty time:year ;
    ] ;
  rdfs:subClassOf [
      a owl:Restriction ;
      owl:hasValue <http://www.opengis.net/def/uom/ISO-8601/0/Gregorian> ;
      owl:onProperty time:hasTRS ;
    ] ;
  skos:definition "Description of date structured with separate values for year and a sub-year grouping such as a season or quarter. The temporal reference system is fixed to Gregorian Calendar and the range of the year property is restricted to xsd:gYear."@en
  .

:decade
  rdf:type owl:DatatypeProperty ;
  rdfs:comment "Decade position in the Gregorian calendar; e.g. 197 is the decade starting with 1970"@en ;
  rdfs:domain :SuperYearDateTimeDescription ;
  rdfs:label "decade"@en ;
  rdfs:range xsd:integer ;
  skos:definition "Decade position in the Gregorian calendar; e.g. 197 is the decade starting with 1970"@en ;
.

:century
  rdf:type owl:DatatypeProperty ;
  rdfs:comment "Century position in the Gregorian calendar; e.g. 19 is the century starting with 1900"@en ;
  rdfs:domain :SuperYearDateTimeDescription ;
  rdfs:label "century"@en ;
  rdfs:range xsd:integer ;
  skos:definition "Century position in the Gregorian calendar; e.g. 19 is the century starting with 1900"@en ;
.

# decade implies century so descriptions should not use both
:decade owl:propertyDisjointWith :century .

:SuperYearDateTimeDescription
  a owl:Class ;
  rdfs:comment "Description of date and time structured with separate values for decade and century for when the date has year precision but a year value is not specified. The temporal reference system is fixed to Gregorian Calendar."@en ;
  rdf:label "Super-year date description"@en ;
  rdfs:subClassOf time:DateTimeDescription ;
  rdfs:subClassOf [
      a owl:Restriction ;
      owl:cardinality "0"^^xsd:nonNegativeInteger ;
      owl:onProperty time:year ;
    ] ;
  rdfs:subClassOf [
      rdf:type owl:Restriction ;
      owl:hasValue :unitYear ;
      owl:onProperty :unitType ;
    ] ;
  rdfs:subClassOf [
    rdf:type owl:Restriction ;
    owl:maxCardinality "1"^^xsd:nonNegativeInteger ;
    owl:onProperty :decade
    ] ;
  rdfs:subClassOf [
    rdf:type owl:Restriction ;
    owl:maxCardinality "1"^^xsd:nonNegativeInteger ;
    owl:onProperty :century
    ] ;
  skos:definition "Description of date and time structured with separate values for decade and century for when a year value is not specified. The temporal reference system is fixed to Gregorian Calendar."@en
  .

:Spring
  a :Season ;
  rdfs:label "Spring"@en ;
  skos:prefLabel "Spring"@en
  .

:SpringNorthernHemisphere
  a :Season ;
  rdfs:label "Spring - Northern Hemisphere"@en ;
  skos:prefLabel "Spring - Northern Hemisphere"@en
  .

:SpringSouthernHemisphere
  a :Season ;
  rdfs:label "Spring - Southern Hemisphere"@en ;
  skos:prefLabel "Spring - Southern Hemisphere"@en
  .

:Summer
  a :Season ;
  rdfs:label "Summer"@en ;
  skos:prefLabel "Summer"@en
  .

:SummerNorthernHemisphere
  a :Season ;
  rdfs:label "Summer - Northern Hemisphere"@en ;
  skos:prefLabel "Summer - Northern Hemisphere"@en
  .

:SummerSouthernHemisphere
  a :Season ;
  rdfs:label "Summer - Southern Hemisphere"@en ;
  skos:prefLabel "Summer - Southern Hemisphere"@en
  .

:Fall
  a :Season ;
  rdfs:label "Fall"@en ;
  skos:prefLabel "Fall"@en
  .

:FallNorthernHemisphere
  a :Season ;
  rdfs:label "Fall - Northern Hemisphere"@en ;
  skos:prefLabel "Fall - Northern Hemisphere"@en
  .

:FallSouthernHemisphere
  a :Season ;
  rdfs:label "Fall - Southern Hemisphere"@en ;
  skos:prefLabel "Fall - Southern Hemisphere"@en
  .

:Winter
  a :Season ;
  rdfs:label "Winter"@en ;
  skos:prefLabel "Winter"@en
  .

:WinterNorthernHemisphere
  a :Season ;
  rdfs:label "Winter - Northern Hemisphere"@en ;
  skos:prefLabel "Winter - Northern Hemisphere"@en
  .

:WinterSouthernHemisphere
  a :Season ;
  rdfs:label "Winter - Southern Hemisphere"@en ;
  skos:prefLabel "Winter - Southern Hemisphere"@en
  .

:Quarter1
  a :Quarter ;
  rdfs:label "Quarter 1"@en ;
  skos:prefLabel "Quarter 1"@en ;
  time:month "--01"^^xsd:gMonth ;
  time:unitType time:unitQuarter
  .

:Quarter2
  a :Quarter ;
  rdfs:label "Quarter 2"@en ;
  skos:prefLabel "Quarter 2"@en ;
  time:month "--04"^^xsd:gMonth ;
  time:unitType time:unitQuarter
  .

:Quarter3
  a :Quarter ;
  rdfs:label "Quarter 3"@en ;
  skos:prefLabel "Quarter 3"@en ;
  time:month "--07"^^xsd:gMonth ;
  time:unitType time:unitQuarter
  .

:Quarter4
  a :Quarter ;
  rdfs:label "Quarter 4"@en ;
  skos:prefLabel "Quarter 4"@en ;
  time:month "--10"^^xsd:gMonth ;
  time:unitType time:unitQuarter
  .

:Quadrimester1
  a :Quadrimester ;
  rdfs:label "Quadrimester 1"@en ;
  skos:prefLabel "Quadrimester 1"@en ;
  time:month "--01"^^xsd:gMonth ;
  time:unitType time:unitQuadrimester
  .

:Quadrimester2
  a :Quadrimester ;
  rdfs:label "Quadrimester 2"@en ;
  skos:prefLabel "Quadrimester 2"@en ;
  time:month "--05"^^xsd:gMonth ;
  time:unitType time:unitQuadrimester
  .

:Quadrimester3
  a :Quadrimester ;
  rdfs:label "Quadrimester 3"@en ;
  skos:prefLabel "Quadrimester 3"@en ;
  time:month "--09"^^xsd:gMonth ;
  time:unitType time:unitQuadrimester
  .

:Semestral1
  a :Semestral ;
  rdfs:label "Semestral 1"@en ;
  skos:prefLabel "Semestral 1"@en ;
  time:month "--01"^^xsd:gMonth ;
  time:unitType time:unitSemestral
  .

:Semestral2
  a :Semestral ;
  rdfs:label "Semestral 2"@en ;
  skos:prefLabel "Semestral 2"@en ;
  time:month "--07"^^xsd:gMonth ;
  time:unitType time:unitSemestral
  .
