@base <https://periodo.github.io/edtf-ontology/edtfo.ttl> .

@prefix : <#> .
@prefix dct: <http://purl.org/dc/terms/> .
@prefix edtf: <http://id.loc.gov/datatypes/edtf/> .
@prefix greg: <http://www.w3.org/ns/time/gregorian/> .
@prefix owl: <http://www.w3.org/2002/07/owl#> .
@prefix rdf: <http://www.w3.org/1999/02/22-rdf-syntax-ns#> .
@prefix rdfs: <http://www.w3.org/2000/01/rdf-schema#> .
@prefix skos: <http://www.w3.org/2004/02/skos/core#> .
@prefix time: <http://www.w3.org/2006/time#> .
@prefix xsd: <http://www.w3.org/2001/XMLSchema#> .

<>
  a owl:Ontology ;
  dct:creator <https://orcid.org/0000-0002-5486-159X> ;
  rdfs:comment "Draft ontology for EDTF concepts."@en ;
  rdfs:label "Extended Date/Time Format (EDTF) concepts"@en ;
  owl:imports <http://www.w3.org/2006/time>
  .

:SubYearDateTimeDescription
  a owl:Class ;
  rdf:label "Sub-year date description"@en ;
  rdfs:subClassOf time:DateTimeDescription ;
  rdfs:subClassOf [
      a owl:Restriction ;
      owl:maxCardinality "1"^^xsd:nonNegativeInteger ;
      owl:onProperty :yearSubdivision ;
    ] ;
  skos:definition """Description of date and time structured with a
separate value for a sub-year grouping such as a season or
quarter. The temporal reference system is fixed to Gregorian
Calendar."""@en ;
  .

:YearSubdivision
  a owl:Class ;
  rdfs:label "Subdivision of year"@en ;
  rdfs:subClassOf owl:Thing ;
  skos:definition "A subdivision of the year"@en ;
  skos:note """Membership of the class :YearSubdivision is open,
to allow for alternative subdivisions."""@en
  .

:Season
  a owl:Class ;
  rdfs:label "Season of year"@en ;
  rdfs:subClassOf :YearSubdivision ;
  rdfs:subClassOf [
      a owl:Restriction ;
      owl:hasValue :unitSeason ;
      owl:onProperty time:unitType ;
    ] ;
  skos:definition "A season of the year"@en ;
  skos:note """Membership of the class :Season is open,
to allow for alternative seasons."""@en
  .

:Quarter
  a owl:Class ;
  rdfs:label "Quarter of year"@en ;
  rdfs:subClassOf :YearSubdivision ;
  rdfs:subClassOf [
      a owl:Restriction ;
      owl:hasValue :unitQuarter ;
      owl:onProperty time:unitType ;
    ] ;
  owl:oneOf (
    :Quarter1
    :Quarter2
    :Quarter3
    :Quarter4
    ) ;
  skos:definition "A quarter of the year"@en
  .

:Quadrimester
  a owl:Class ;
  rdfs:label "Quadrimester of year"@en ;
  rdfs:subClassOf :YearSubdivision ;
  rdfs:subClassOf [
      a owl:Restriction ;
      owl:hasValue :unitQuadrimester ;
      owl:onProperty time:unitType ;
    ] ;
  owl:oneOf (
    :Quadrimester1
    :Quadrimester2
    :Quadrimester3
    ) ;
  skos:definition "A quadrimester of the year"@en
  .

:Semestral
  a owl:Class ;
  rdfs:label "Semestral of year"@en ;
  rdfs:subClassOf :YearSubdivision ;
  rdfs:subClassOf [
      a owl:Restriction ;
      owl:hasValue :unitSemestral ;
      owl:onProperty time:unitType ;
    ] ;
  owl:oneOf (
    :Semestral1
    :Semestral2
    ) ;
  skos:definition "A semestral of the year"@en
  .

:SuperYearDateTimeDescription
  a owl:Class ;
  rdf:label "Super-year date description"@en ;
  rdfs:subClassOf time:DateTimeDescription ;
  rdfs:subClassOf [
    a owl:Restriction ;
    owl:cardinality "0"^^xsd:nonNegativeInteger ;
    owl:onProperty time:year ;
    ] ;
  skos:definition """Description of date and time structured with
  separate values for decade or century or millennium, for when the
  date has <= year precision but a year value is not specified. The
  temporal reference system is fixed to Gregorian Calendar."""@en
  .

:DecadeDescription
  a owl:Class ;
  rdf:label "Decade description"@en ;
  rdfs:subClassOf :SuperYearDateTimeDescription ;
  rdfs:subClassOf [
    a owl:Restriction ;
    owl:maxCardinality "1"^^xsd:nonNegativeInteger ;
    owl:onProperty :decade
    ]
  .

:CenturyDescription
  a owl:Class ;
  rdf:label "Century description"@en ;
  rdfs:subClassOf :SuperYearDateTimeDescription ;
  rdfs:subClassOf [
    a owl:Restriction ;
    owl:maxCardinality "1"^^xsd:nonNegativeInteger ;
    owl:onProperty :century
    ]
  .

:MillenniumDescription
  a owl:Class ;
  rdf:label "Millennium description"@en ;
  rdfs:subClassOf :SuperYearDateTimeDescription ;
  rdfs:subClassOf [
    a owl:Restriction ;
    owl:maxCardinality "1"^^xsd:nonNegativeInteger ;
    owl:onProperty :millennium
    ]
  .

[] a owl:AllDisjointClasses ;
  owl:members (
  :DecadeDescription
  :CenturyDescription
  :MillenniumDescription
    )
  .

:OpenEndInterval
  a owl:Class ;
  rdfs:label "Open end interval"@en ;
  rdfs:subClassOf time:ProperInterval ;
  rdfs:subClassOf [
    a owl:Restriction ;
    owl:cardinality "0"^^xsd:nonNegativeInteger ;
    owl:onProperty time:hasEnd ;
    ] ;
  skos:definition """A temporal entity with non-zero extent or duration
  and for which the value of the end is unspecified (perhaps because
  it does not exist but not because it is unknown)"""@en ;
  .

:OpenBeginningInterval
  a owl:Class ;
  rdfs:label "Open beginning interval"@en ;
  rdfs:subClassOf time:ProperInterval ;
  rdfs:subClassOf [
    a owl:Restriction ;
    owl:cardinality "0"^^xsd:nonNegativeInteger ;
    owl:onProperty time:hasBeginning ;
    ] ;
  skos:definition """A temporal entity with non-zero extent or duration
  and for which the value of the beginning is unspecified (perhaps
  because it does not exist but not because it is unknown)"""@en
  .

:QualifiedStatement
  a owl:Class ;
  rdfs:label "Qualified statement"@en ;
  rdfs:subClassOf rdf:Statement ;
  skos:definition "A qualified (e.g. uncertain or approximate) statement"@en
  .

:UncertainStatement
  a owl:Class ;
  rdfs:label "Uncertain statement"@en ;
  rdfs:subClassOf :QualifiedStatement ;
  skos:definition "An uncertain statement"@en
  .

:ApproximateStatement
  a owl:Class ;
  rdfs:label "Approximate statement"@en ;
  rdfs:subClassOf :QualifiedStatement ;
  skos:definition "An approximate statement"@en
  .

:yearSubdivision
  a owl:ObjectProperty ;
  rdfs:domain :SubYearDateDescription ;
  rdfs:label "year subdivision"@en ;
  rdfs:range :YearSubdivision ;
  skos:definition """The subdivision of the year,
whose value is a member of the class edtfo:YearSubdivision"""@en
  .

:hasEDTFDateTimeDescription
  a owl:DatatypeProperty ;
  rdfs:domain time:Interval ;
  rdfs:label "has EDTF datetime description"@en ;
  rdfs:range edtf:EDTF ;
  skos:definition "Value of an interval, expressed using EDTF"@en
  .

:hasEDTFDateTimeSetDescription
  a owl:DatatypeProperty ;
  rdfs:domain owl:Class ;
  rdfs:label "has EDTF datetime set description"@en ;
  rdfs:range edtf:EDTF-level2 ;
  skos:definition """Value of a set of instants, expressed using EDTF

This property is intended for use with EDTF level 2 “all members of set”
(curly brackets) notation. For “one of a set” expressions use
edtfo:inEDTFDateTime.
"""@en
  .

:inEDTFDateTime
  a owl:DatatypeProperty ;
  rdfs:domain time:Instant ;
  rdfs:label "in EDTF datetime"@en ;
  rdfs:range edtf:EDTF ;
  skos:definition "Position of an instant, expressed using EDTF"@en
  .

:decade
  a owl:DatatypeProperty ;
  rdfs:domain :DecadeDescription ;
  rdfs:label "decade"@en ;
  rdfs:range xsd:integer ;
  skos:definition """Decade position in the Gregorian calendar;
e.g. 197 is the decade starting with 1970"""@en
  .

:century
  a owl:DatatypeProperty ;
  rdfs:domain :CenturyDescription ;
  rdfs:label "century"@en ;
  rdfs:range xsd:integer ;
  skos:definition """Century position in the Gregorian calendar;
e.g. 19 is the century starting with 1900"""@en
  .

:millennium
  a owl:DatatypeProperty ;
  rdfs:domain :MillenniumDescription ;
  rdfs:label "millennium"@en ;
  rdfs:range xsd:integer ;
  skos:definition """Millennium position in the Gregorian calendar;
e.g. 1 is the century starting with 1000"""@en
  .

edtf:EDTF
  a owl:Datatype ;
  rdfs:label "Extended Date/Time Format"@en ;
  skos:definition """This datatype describes a date and time
that adheres to features of EDTF Levels 0, 1, and 2."""@en
  .

edtf:EDTF-level0
  a owl:Datatype ;
  rdfs:subClassOf edtf:EDTF;
  rdfs:label "Extended Date/Time Format - Level 0"@en ;
  owl:onDatatype xsd:string ;
  owl:withRestrictions ([
      xsd:pattern ".*" # TODO
      ]) ;
  skos:definition """Level 0 features describe dates, dates and times,
and intervals. The latter are represented by start and end
dates. Level 0 supports ISO 8601 features and could be considered a
profile of ISO 8601."""@en
  .

edtf:EDTF-level1
  a owl:Datatype ;
  rdfs:subClassOf edtf:EDTF;
  rdfs:label "Extended Date/Time Format - Level 1"@en ;
  owl:onDatatype xsd:string ;
  owl:withRestrictions ([
      xsd:pattern ".*" # TODO
      ]) ;
  skos:definition """Level 1 features describe uncertain, approximate, or
unspecified dates, including provisions for intervals."""@en
  .

edtf:EDTF-level2
  a owl:Datatype ;
  rdfs:subClassOf edtf:EDTF;
  rdfs:label "Extended Date/Time Format - Level 2"@en ;
  owl:onDatatype xsd:string ;
  owl:withRestrictions ([
      xsd:pattern ".*" # TODO
      ]) ;
  skos:definition """Level 2 features provide a way to describe dates that
have elements, such as days or months, that are known but which also
have elements that are uncertain, approximate, or unspecified. Level
2 also describes dates that are part of a set."""@en
  .

:unitSeason
  a time:TemporalUnit , owl:NamedIndividual ;
  rdfs:label "Season (unit of temporal duration)"@en ;
  skos:prefLabel "season"@en
  .

:unitQuarter
  a time:TemporalUnit , owl:NamedIndividual ;
  rdfs:label "Quarter (unit of temporal duration equivalent to 3 months)"@en ;
  skos:prefLabel "quarter"@en ;
  time:days "0"^^xsd:decimal ;
  time:hours "0"^^xsd:decimal ;
  time:minutes "0"^^xsd:decimal ;
  time:months "3"^^xsd:decimal ;
  time:seconds "0"^^xsd:decimal ;
  time:weeks "0"^^xsd:decimal ;
  time:years "0"^^xsd:decimal
  .

:unitQuadrimester
  a time:TemporalUnit , owl:NamedIndividual ;
  rdfs:label """Quadrimester (unit of temporal duration
equivalent to 4 months)"""@en ;
  skos:prefLabel "quadrimester"@en ;
  time:days "0"^^xsd:decimal ;
  time:hours "0"^^xsd:decimal ;
  time:minutes "0"^^xsd:decimal ;
  time:months "4"^^xsd:decimal ;
  time:seconds "0"^^xsd:decimal ;
  time:weeks "0"^^xsd:decimal ;
  time:years "0"^^xsd:decimal
  .

:unitSemestral
  a time:TemporalUnit , owl:NamedIndividual ;
  rdfs:label "Semestral (unit of temporal duration equivalent to 6 months)"@en ;
  skos:prefLabel "semestral"@en ;
  time:days "0"^^xsd:decimal ;
  time:hours "0"^^xsd:decimal ;
  time:minutes "0"^^xsd:decimal ;
  time:months "6"^^xsd:decimal ;
  time:seconds "0"^^xsd:decimal ;
  time:weeks "0"^^xsd:decimal ;
  time:years "0"^^xsd:decimal
  .

:Spring
  a :Season , owl:NamedIndividual ;
  rdfs:label "Spring"@en
  .

:SpringNorthernHemisphere
  a :Season , owl:NamedIndividual ;
  rdfs:label "Spring - Northern Hemisphere"@en
  .

:SpringSouthernHemisphere
  a :Season , owl:NamedIndividual ;
  rdfs:label "Spring - Southern Hemisphere"@en
  .

:Summer
  a :Season , owl:NamedIndividual ;
  rdfs:label "Summer"@en
  .

:SummerNorthernHemisphere
  a :Season , owl:NamedIndividual ;
  rdfs:label "Summer - Northern Hemisphere"@en
  .

:SummerSouthernHemisphere
  a :Season , owl:NamedIndividual ;
  rdfs:label "Summer - Southern Hemisphere"@en
  .

:Fall
  a :Season , owl:NamedIndividual ;
  rdfs:label "Fall"@en
  .

:FallNorthernHemisphere
  a :Season , owl:NamedIndividual ;
  rdfs:label "Fall - Northern Hemisphere"@en
  .

:FallSouthernHemisphere
  a :Season , owl:NamedIndividual ;
  rdfs:label "Fall - Southern Hemisphere"@en
  .

:Winter
  a :Season , owl:NamedIndividual ;
  rdfs:label "Winter"@en ;
  skos:prefLabel "Winter"@en
  .

:WinterNorthernHemisphere
  a :Season , owl:NamedIndividual ;
  rdfs:label "Winter - Northern Hemisphere"@en
  .

:WinterSouthernHemisphere
  a :Season , owl:NamedIndividual ;
  rdfs:label "Winter - Southern Hemisphere"@en
  .

:Quarter1
  a :Quarter , owl:NamedIndividual ;
  rdfs:label "Quarter 1"@en ;
  time:month "--01"^^xsd:gMonth ;
  time:unitType :unitQuarter
  .

:Quarter2
  a :Quarter , owl:NamedIndividual ;
  rdfs:label "Quarter 2"@en ;
  time:month "--04"^^xsd:gMonth ;
  time:unitType :unitQuarter
  .

:Quarter3
  a :Quarter , owl:NamedIndividual ;
  rdfs:label "Quarter 3"@en ;
  time:month "--07"^^xsd:gMonth ;
  time:unitType :unitQuarter
  .

:Quarter4
  a :Quarter , owl:NamedIndividual ;
  rdfs:label "Quarter 4"@en ;
  time:month "--10"^^xsd:gMonth ;
  time:unitType :unitQuarter
  .

:Quadrimester1
  a :Quadrimester , owl:NamedIndividual ;
  rdfs:label "Quadrimester 1"@en ;
  time:month "--01"^^xsd:gMonth ;
  time:unitType :unitQuadrimester
  .

:Quadrimester2
  a :Quadrimester , owl:NamedIndividual ;
  rdfs:label "Quadrimester 2"@en ;
  time:month "--05"^^xsd:gMonth ;
  time:unitType :unitQuadrimester
  .

:Quadrimester3
  a :Quadrimester , owl:NamedIndividual ;
  rdfs:label "Quadrimester 3"@en ;
  time:month "--09"^^xsd:gMonth ;
  time:unitType :unitQuadrimester
  .

:Semestral1
  a :Semestral , owl:NamedIndividual ;
  rdfs:label "Semestral 1"@en ;
  time:month "--01"^^xsd:gMonth ;
  time:unitType :unitSemestral
  .

:Semestral2
  a :Semestral , owl:NamedIndividual ;
  rdfs:label "Semestral 2"@en ;
  time:month "--07"^^xsd:gMonth ;
  time:unitType :unitSemestral
  .
